src/MemClass.v
@@ -1,6 +1,5 @@
 Require Export Mem.
 Require Import Word.
-Require Import Basics.
 
 Set Implicit Arguments.
 
@@ -15,7 +14,7 @@ Proof.
   destruct a, b; auto.
 Defined.
 
-Definition single_mem V := @mem unit _ (const V).
+Definition single_mem V := @mem unit _ V.
 
 Definition singleton V (v:V) : single_mem V :=
   fun _ => Some v.
@@ -25,8 +24,8 @@ Module Example.
   Definition addrlen := 64.
   Notation addr := (word addrlen).
 
-  Definition addr_mem := @mem addr _ (fun _ => unit).
-  Definition nat_mem := @mem nat _ (fun _ => unit).
+  Definition addr_mem := @mem addr _ unit.
+  Definition nat_mem := @mem nat _ unit.
 End Example.
 
 Instance pair_dec : forall A B, EqDec A -> EqDec B -> EqDec (A*B).
